fixing jal

SP1Chips/JalChip.lean
@@ -2,6 +2,10 @@ import SP1Operations.Operation.AddOperation
 
 namespace JalChip
 
+open BitVec
+
+open Sail SailState BitVec LeanRV64IM.Functions
+
 def constraints (Main : Vector (Fin BB) 31) : SP1ConstraintList :=
   let E0 : Fin BB := Main[30] - 1
   let E1 : Fin BB := Main[30] * E0
@@ -67,343 +71,224 @@ def constraints (Main : Vector (Fin BB) 31) : SP1ConstraintList :=
 
 open LeanRV64IM.Functions
 
-lemma eq_zero_of_constraints (Main : Vector (Fin BB) 31)
-    (h_cstrs : (constraints Main).allHold) : Main[25] = 0 := by
-  simp [constraints] at h_cstrs
-  aesop
+-- lemma eq_zero_of_constraints (Main : Vector (Fin BB) 31)
+--     (h_cstrs : (constraints Main).allHold) : Main[25] = 0 := by
+--   simp [constraints] at h_cstrs
+--   aesop
 
-lemma isU64_of_constraints (Main : Vector (Fin BB) 31)
-    (h_cstrs : (constraints Main).allHold)
-    (h_is_real : Main[30] = 1) :
-    Word.isU64 #v[Main[3], Main[4], Main[5], 0] := by
-  simp [constraints, h_is_real, SP1Constraint.toProp] at h_cstrs
-  refine Word.isU64_of_cases ?_ ?_ ?_ ?_ ?_
-  · aesop
-  · aesop
-  · aesop
-  · aesop
+-- lemma isU64_of_constraints (Main : Vector (Fin BB) 31)
+--     (h_cstrs : (constraints Main).allHold)
+--     (h_is_real : Main[30] = 1) :
+--     Word.isU64 #v[Main[3], Main[4], Main[5], 0] := by
+--   simp [constraints, h_is_real, SP1Constraint.toProp] at h_cstrs
+--   refine Word.isU64_of_cases ?_ ?_ ?_ ?_ ?_
+--   · aesop
+--   · aesop
+--   · aesop
+--   · aesop
 
-lemma isU64_of_constraints' (Main : Vector (Fin BB) 31)
-    (h_cstrs : (constraints Main).allHold)
-    (h_is_real : Main[30] = 1) :
-    Word.isU64 #v[Main[14], Main[15], Main[16], Main[17]] := by
-  simp [constraints, h_is_real, SP1Constraint.toProp] at h_cstrs
-  refine Word.isU64_of_cases ?_ ?_ ?_ ?_ ?_
-  · aesop
-  · aesop
-  · aesop
-  · aesop
+-- lemma isU64_of_constraints' (Main : Vector (Fin BB) 31)
+--     (h_cstrs : (constraints Main).allHold)
+--     (h_is_real : Main[30] = 1) :
+--     Word.isU64 #v[Main[14], Main[15], Main[16], Main[17]] := by
+--   simp [constraints, h_is_real, SP1Constraint.toProp] at h_cstrs
+--   refine Word.isU64_of_cases ?_ ?_ ?_ ?_ ?_
+--   · aesop
+--   · aesop
+--   · aesop
+--   · aesop
 
-lemma program_constraints_allHold (Main : Vector (Fin BB) 31)
-    (h_cstrs : (constraints Main).allHold) :
-    SP1Constraint.toProp (.send (.program Main[3] Main[4] Main[5] (Opcode.ofNat 33)
-      Main[6] Main[14] Main[15] Main[16] Main[17] Main[18] Main[19]
-      Main[20] Main[21] Main[13] 1 1 111 0 0) Main[30]) := by
-  simp [constraints] at h_cstrs
-  aesop
+-- lemma program_constraints_allHold (Main : Vector (Fin BB) 31)
+--     (h_cstrs : (constraints Main).allHold) :
+--     SP1Constraint.toProp (.send (.program Main[3] Main[4] Main[5] (Opcode.ofNat 33)
+--       Main[6] Main[14] Main[15] Main[16] Main[17] Main[18] Main[19]
+--       Main[20] Main[21] Main[13] 1 1 111 0 0) Main[30]) := by
+--   simp [constraints] at h_cstrs
+--   aesop
 
-lemma link_eq_of_constraints (Main : Vector (Fin BB) 31)
-    (h_cstrs : (constraints Main).allHold)
-    (h_is_real : Main[30] = 1) (h_op_a : Main[13] = 0) :
-    BitVec.ofNat 64 (Main[26] + Main[27] * 2^16 + Main[28] * 2^32 +  Main[29] * 2^48) =
-      BitVec.ofNat 64 (Main[3] + Main[4] * 2^16 + Main[5] * 2^32) + 4 := by
-  have h345 := isU64_of_constraints Main h_cstrs h_is_real
-  simp [constraints] at h_cstrs
-  have : (AddOperation.constraints #v[Main[3], Main[4], Main[5], 0] #v[4, 0, 0, 0]
-      { value := #v[Main[26], Main[27], Main[28], Main[29]] } (Main[30] - Main[13])).allHold := by
-    aesop
-  have := AddOperation.correct _ _ _ _ ?_ this h345 ?_
-  simp [Word.toBitVec64] at this
-  have := this.2
-  refine this.trans ?_
-  simp [Word.toNat]
-  · simp [h_op_a, h_is_real]
-  · apply Word.isU64_of_cases <;> simp
+-- lemma link_eq_of_constraints (Main : Vector (Fin BB) 31)
+--     (h_cstrs : (constraints Main).allHold)
+--     (h_is_real : Main[30] = 1) (h_op_a : Main[13] = 0) :
+--     BitVec.ofNat 64 (Main[26] + Main[27] * 2^16 + Main[28] * 2^32 +  Main[29] * 2^48) =
+--       BitVec.ofNat 64 (Main[3] + Main[4] * 2^16 + Main[5] * 2^32) + 4 := by
+--   have h345 := isU64_of_constraints Main h_cstrs h_is_real
+--   simp [constraints] at h_cstrs
+--   have : (AddOperation.constraints #v[Main[3], Main[4], Main[5], 0] #v[4, 0, 0, 0]
+--       { value := #v[Main[26], Main[27], Main[28], Main[29]] } (Main[30] - Main[13])).allHold := by
+--     aesop
+--   have := AddOperation.correct _ _ _ _ ?_ this h345 ?_
+--   simp [Word.toBitVec64] at this
+--   have := this.2
+--   refine this.trans ?_
+--   simp [Word.toNat]
+--   · simp [h_op_a, h_is_real]
+--   · apply Word.isU64_of_cases <;> simp
 
-lemma add_imm_eq_of_constarints (Main : Vector (Fin BB) 31)
-    (h_cstrs : (constraints Main).allHold)
-    (h_is_real : Main[30] = 1) :
-    BitVec.ofNat 64 (Main[22] + Main[23] * 65536 + Main[24] * 4294967296) =
-        BitVec.ofNat 64 (Main[3] + Main[4] * 65536 + ↑Main[5] * 4294967296) +
-          BitVec.ofNat 64 (Main[14] + Main[15] * 65536 + Main[16] * 4294967296 + Main[17] * 281474976710656) := by
-  have h345 := isU64_of_constraints Main h_cstrs h_is_real
-  have h1415 := isU64_of_constraints' Main h_cstrs h_is_real
-  simp [constraints] at h_cstrs
-  have : (AddOperation.constraints #v[Main[3], Main[4], Main[5], 0] #v[Main[14], Main[15], Main[16], Main[17]]
-      { value := #v[Main[22], Main[23], Main[24], Main[25]] } Main[30]).allHold := by
-    aesop
-  have := AddOperation.correct _ _ _ _ h_is_real this h345 h1415
-  simp [Word.toBitVec64] at this
-  have := this.2
-  have h25 : Main[25] = 0 := h_cstrs.2.1
-  simp [Word.toNat, h25] at this
-  exact this
+-- lemma add_imm_eq_of_constarints (Main : Vector (Fin BB) 31)
+--     (h_cstrs : (constraints Main).allHold)
+--     (h_is_real : Main[30] = 1) :
+--     BitVec.ofNat 64 (Main[22] + Main[23] * 65536 + Main[24] * 4294967296) =
+--         BitVec.ofNat 64 (Main[3] + Main[4] * 65536 + ↑Main[5] * 4294967296) +
+--           BitVec.ofNat 64 (Main[14] + Main[15] * 65536 + Main[16] * 4294967296 + Main[17] * 281474976710656) := by
+--   have h345 := isU64_of_constraints Main h_cstrs h_is_real
+--   have h1415 := isU64_of_constraints' Main h_cstrs h_is_real
+--   simp [constraints] at h_cstrs
+--   have : (AddOperation.constraints #v[Main[3], Main[4], Main[5], 0] #v[Main[14], Main[15], Main[16], Main[17]]
+--       { value := #v[Main[22], Main[23], Main[24], Main[25]] } Main[30]).allHold := by
+--     aesop
+--   have := AddOperation.correct _ _ _ _ h_is_real this h345 h1415
+--   simp [Word.toBitVec64] at this
+--   have := this.2
+--   have h25 : Main[25] = 0 := h_cstrs.2.1
+--   simp [Word.toNat, h25] at this
+--   exact this
 
-/-- dt: should extract this out and clean up more -/
-lemma ofInt_ofNat_of_constraints (Main : Vector (Fin BB) 31)
-    (h_cstrs : (constraints Main).allHold)
-    (h_is_real : Main[30] = 1) :
-    let imm_nat : ℕ := Main[14] + Main[15] * 65536 + Main[16] * 4294967296 + Main[17] * 281474976710656
-    BitVec.ofInt 64 (BitVec.ofNat 21 (imm_nat)).toInt = (BitVec.ofNat 64 (imm_nat)) := by
-  have := program_constraints_allHold Main h_cstrs
-  simp [SP1Constraint.toProp, h_is_real, Opcode.ofNat, Nat.ble] at this
+-- /-- dt: should extract this out and clean up more -/
+-- lemma ofInt_ofNat_of_constraints (Main : Vector (Fin BB) 31)
+--     (h_cstrs : (constraints Main).allHold)
+--     (h_is_real : Main[30] = 1) :
+--     let imm_nat : ℕ := Main[14] + Main[15] * 65536 + Main[16] * 4294967296 + Main[17] * 281474976710656
+--     BitVec.ofInt 64 (BitVec.ofNat 21 (imm_nat)).toInt = (BitVec.ofNat 64 (imm_nat)) := by
+--   have := program_constraints_allHold Main h_cstrs
+--   simp [SP1Constraint.toProp, h_is_real, Opcode.ofNat, Nat.ble] at this
 
-  obtain ⟨⟨h14, h15, h16, h17⟩, _⟩ := this.1
-  simp [h15, h16, h17]
-  simp [BitVec.ofInt, BitVec.toInt]
-  simp [Int.toNat]
+--   obtain ⟨⟨h14, h15, h16, h17⟩, _⟩ := this.1
+--   simp [h15, h16, h17]
+--   simp [BitVec.ofInt, BitVec.toInt]
+--   simp [Int.toNat]
 
-  have h14' : Main[14].val % 2097152 = Main[14].val
-  · rw [Nat.mod_eq_of_lt]
-    omega
-  have h14'' : (Main[14].val : ℤ) % (2097152 : ℤ) = Main[14].val
-  · exact
-    Eq.symm
-      ((fun {a b} ↦ Int.neg_inj.mp) (congrArg Neg.neg (congrArg Nat.cast (id (Eq.symm h14')))))
-  simp [h14', h14'']
-  have h14''' : 2 * Main[14].val < 2097152 := by omega
-  simp [h14''']
-  rename_i right
-  simp_all only [SP1ConstraintList.allHold, BB_eq, Fin.isValue, and_self, Fin.reduceLT, and_true, true_and]
-  obtain ⟨left, right_1⟩ := this
-  obtain ⟨left_2, right_1⟩ := right_1
-  obtain ⟨left_3, right_1⟩ := right_1
-  obtain ⟨left_5, right_1⟩ := right_1
-  simp_all only [Fin.isValue]
-  rfl
+--   have h14' : Main[14].val % 2097152 = Main[14].val
+--   · rw [Nat.mod_eq_of_lt]
+--     omega
+--   have h14'' : (Main[14].val : ℤ) % (2097152 : ℤ) = Main[14].val
+--   · exact
+--     Eq.symm
+--       ((fun {a b} ↦ Int.neg_inj.mp) (congrArg Neg.neg (congrArg Nat.cast (id (Eq.symm h14')))))
+--   simp [h14', h14'']
+--   have h14''' : 2 * Main[14].val < 2097152 := by omega
+--   simp [h14''']
+--   rename_i right
+--   simp_all only [SP1ConstraintList.allHold, BB_eq, Fin.isValue, and_self, Fin.reduceLT, and_true, true_and]
+--   obtain ⟨left, right_1⟩ := this
+--   obtain ⟨left_2, right_1⟩ := right_1
+--   obtain ⟨left_3, right_1⟩ := right_1
+--   obtain ⟨left_5, right_1⟩ := right_1
+--   simp_all only [Fin.isValue]
+--   rfl
 
 --------------------------
 
-def specJal (imm : BitVec 21) (rd : regidx) : SailM Unit := do
-  set_next_pc (Sail.BitVec.addInt (← Sail.readReg Register.PC) 4)
-  let _ ← execute_JAL imm rd
+lemma op_a_lt32_of_constraints {Main : Vector (Fin BB) 31}
+    (h_cstrs : (constraints Main).allHold)
+    (h_is_real : Main[30] = 1) : Main[6].val < 32 := by
+  simp only [BB_eq, Nat.reducePow]
+  simp [SP1ConstraintList.allHold, constraints, SP1Constraint.toProp] at h_cstrs
+  have h : Main[6] < 32 := by aesop
+  clear h_cstrs
+  aesop
 
-def sp1Jal (Main : Vector (Fin BB) 31) : SailM Unit := do
+variable (Main : Vector (Fin BB) 31)
+  (s : SailState) (cstrs : (constraints Main).allHold)
+  (h_is_real : Main[30] = 1)
+
+def sp1_imm : BitVec 12 := BitVec.ofNat 12 Main[21].val
+
+def sp1_op_a : BitVec 5 := Main[6].val#'(op_a_lt32_of_constraints cstrs h_is_real)
+
+def sp1_jal (Main : Vector (Fin BB) 31) : SailM Unit := do
   let rd := regidx.Regidx Main[6].val
   let new_pc := BitVec.ofNat 64 (Main[22] + Main[23] * 2^16 + Main[24] * 2^32 + Main[25] * 2^48)
   let link := BitVec.ofNat 64 (Main[26] + Main[27] * 2^16 + Main[28] * 2^32 +  Main[29] * 2^48)
   wX_bits rd link
   set_next_pc new_pc
 
--- lemma execute_JAL_eq_of (imm : BitVec 21) (rd : regidx)
---     (s : PreSail.SequentialState RegisterType Sail.trivialChoiceSource)
---     (pc : RegisterType Register.PC) (h : (pc + sign_extend imm) % 4 = 0)
---     (hs : s.regs.get? Register.PC = pc) :
---     (execute_JAL imm rd).run s = (do
---       let target ← pure ((← Sail.readReg Register.PC) + (sign_extend (m := 64) imm))
---       wX_bits rd (← (get_next_pc ()))
---       (set_next_pc target)
---       (pure RETIRE_SUCCESS)).run s := by
---   rw [execute_JAL]
---   simp [ext_control_check_pc, bit_to_bool]
---   simp [Sail.BitVec.access, bits_of_virtaddr]
---   simp [bool_bit_backwards, BitVec.ofBool]
---   sorry
-  -- rw [readReg_bind_bind_duplicate]
-  -- have := run_readReg_bind_of_forall
-  --   (reg := Register.PC)
-  --   (f := fun v => (v + sign_extend imm)[1])
-  --   (y := false)
-  --   (mx := fun b : Bool => do
-  --     let v' ← Sail.readReg Register.PC
-  --     let x ←
-  --       (match bif b then 1#1 else 0#1 with
-  --         | 1#1 => pure true
-  --         | 0#1 => pure false
-  --         | x => do
-  --           Sail.assert false "Pattern match failure at unknown location"
-  --           throw Sail.Error.Exit)
-  --     let __do_lift ← currentlyEnabled extension.Ext_Zca
-  --     bif x && LeanRV64IM.Functions.not __do_lift then
-  --         pure
-  --           (ExecutionResult.Memory_Exception
-  --             (virtaddr.Virtaddr (v' + sign_extend imm), ExceptionType.E_Fetch_Addr_Align ()))
-  --       else do
-  --         let __do_lift ← get_next_pc ()
-  --         wX_bits rd __do_lift
-  --         (fun a ↦ RETIRE_SUCCESS) <$> set_next_pc (v' + sign_extend imm))
-  -- erw [this]
-  -- · simp
-  --   simp [currentlyEnabled]
-  --   refine congr_arg (EStateM.run · s) ?_
-  --   refine bind_congr fun v => ?_
-  --   exact readReg_bind_const Register.misa (do
-  --     let __do_lift ← get_next_pc ()
-  --     wX_bits rd __do_lift
-  --     (fun a ↦ RETIRE_SUCCESS) <$> set_next_pc (v + sign_extend imm))
-  -- · intro v
-  --   simp [hs]
-  --   rintro rfl
-  --   have := BitVec.mul4_means_0_1_are_0 h
-  --   exact this.2
-
--- lemma specJal_eq_of_mod (imm : BitVec 21) (rd : regidx)
---     (s : PreSail.SequentialState RegisterType Sail.trivialChoiceSource)
---     (pc : RegisterType Register.PC)
---     (h : (pc + sign_extend imm) % 4 = 0)
---     (hs : s.regs.get? Register.PC = pc) :
-
---     (specJal imm rd).run s = (do
---       set_next_pc (Sail.BitVec.addInt pc 4)
---       let target ← pure (pc + (sign_extend (m := 64) imm))
---       wX_bits rd (← (get_next_pc ()))
---       (set_next_pc target)).run s := by
---   rw [specJal]
---   simp [EStateM.run_bind]
---   stop
---   have : Sail.readReg Register.PC s = EStateM.Result.ok pc s := sorry
---   simp [this]
---   cases set_next_pc (Sail.BitVec.addInt pc 4) s
---   ·
---     simp
---     simp [EStateM.Result.map]
---     rw [execute_JAL_eq_of imm rd _ pc h]
-
---     · simp [EStateM.run_bind]
-
---       sorry
---     ·
---       sorry
---   simp
-
--- set_option debug.skipKernelTC true in
--- set_option maxHeartbeats 300000 in
--- theorem SP1JAL_correct (Main : Vector (Fin BB) 31)
---     (h_cstrs : (constraints Main).allHold)
---     (h_is_real : Main[30] = 1) -- Is a real column
---     (s : PreSail.SequentialState RegisterType Sail.trivialChoiceSource)
---     -- dt: get this from constraints
---     (h_pc : s.regs.get? Register.PC =
---       some (BitVec.ofNat 64 (Main[3] + Main[4] * 2^16 + Main[5] * 2^32)))
---     (h_misa : s.regs.get? Register.misa = some 2)
---     :
---     let imm := BitVec.ofNat 64 (Main[14] + Main[15] * 2^16 + Main[16] * 2^32 + Main[17] * 2^48)
---     (sp1Jal Main).run s = (specJal imm (regidx.Regidx Main[6].val)).run s := by
+def spec_jal (imm : BitVec 21) (rd : regidx) : SailM Unit := do
+  Sail.writeReg Register.nextPC ((← Sail.readReg Register.PC) + 4#64)
+  let _ ← execute_JAL imm rd
 
 --   let init_pc := BitVec.ofNat 64 (Main[3] + Main[4] * 2^16 + Main[5] * 2^32)
 --   let imm := BitVec.ofNat 64 (Main[14] + Main[15] * 2^16 + Main[16] * 2^32 + Main[17] * 2^48)
 --   let new_pc := BitVec.ofNat 64 (Main[22] + Main[23] * 2^16 + Main[24] * 2^32 + Main[25] * 2^48)
 --   let link := BitVec.ofNat 64 (Main[26] + Main[27] * 2^16 + Main[28] * 2^32 +  Main[29] * 2^48)
 
---   unfold sp1Jal
+set_option debug.skipKernelTC true in
+set_option maxHeartbeats 0 in
+theorem SP1JAL_correct
+    (state_cstrs : (constraints Main).initialState s)
+    (h_misa : Register.misa ∈ s.regs) :
+    let imm := sp1_imm Main
+    let op_a := sp1_op_a Main cstrs h_is_real
+    (spec_jal imm (.Regidx op_a)).run s = (sp1_jal Main).run s := by
+  extract_lets imm op_a
+
+  simp [SP1ConstraintList.initialState, constraints, SP1Constraint.toStateProp, List.Forall, AddOperation.constraints, h_is_real] at state_cstrs
+  obtain ⟨read_pc, h⟩ := state_cstrs
+
+  have h_op_a : Main[6].val < 32 := op_a_lt32_of_constraints cstrs h_is_real
+  specialize h (by aesop)
+
+  simp [SP1ConstraintList.allHold, constraints, SP1Constraint.toProp, sub_eq_zero,
+    h_is_real] at cstrs
+
+  have h_misa' : ∃ v_misa, s.regs.get? Register.misa = some v_misa := by
+
+    sorry
+
+  have hmod : (BitVec.ofNat 64 (↑Main[3] + ↑Main[4] * 65536 + ↑Main[5] * 4294967296) +
+                sign_extend (setWidth 21 (BitVec.ofNat 12 ↑Main[21])))[1] = false := by
+    sorry
+
+  simp [spec_jal, sp1_jal, execute_JAL, op_a, imm, sp1_imm, sp1_op_a]
 
 
---   -- refine _root_.trans ?_ (specJal_eq_of_mod _ _ _ init_pc (by
---   --   simp
+  have h13_is_bool : Main[13] = 0 ∨ Main[13] = 1 := by
+    aesop
 
---   --   sorry
---   -- ) (h_pc)).symm
---   -- refine congr_arg (fun mx => EStateM.run mx s) ?_
---   unfold specJal
---   unfold execute_JAL
+  simp [run_rX_bits, get_reg?_insert_nextPC, ext_control_check_addr, ext_control_check_pc,
+    Sail.BitVec.access, bit_to_bool, Sail.BitVec.update, Sail.BitVec.updateSubrange',
+    bits_of_virtaddr, BitVec.reduceAllOnes, BitVec.truncate_eq_setWidth, BitVec.reduceSetWidth,
+    BitVec.shiftLeft_zero, BitVec.reduceNot, BitVec.setWidth_zero, BitVec.or_zero,
+    Nat.one_lt_ofNat, getElem!_pos, BitVec.getElem_and, BitVec.reduceGetElem, Bool.true_and,
+    BitVec.ofBool, BitVec.ofNat_eq_ofNat, cond_false, EStateM.run_bind,
+    run_bool_bit_backwards, Bool.false_and, EStateM.run_map, run_writeReg, EStateM.Result.map_ok,
+    currentlyEnabled, hartSupports, Bool.false_and, Bool.false_or, Bool.and_self,
+    BitVec.ofNat_eq_ofNat, bind_pure_comp, Functor.map_map, EStateM.run_map]
 
---   simp only [BB_eq, BitVec.natCast_eq_ofNat, Nat.reducePow, Nat.reduceLeDiff,
---     BitVec.setWidth_ofNat_of_le, pure_bind]
+  have h_add : BitVec.ofNat 64 (↑Main[3] + ↑Main[4] * 65536 + ↑Main[5] * 4294967296) +
+      sign_extend (setWidth 21 (BitVec.ofNat 12 ↑Main[21])) =
+      (BitVec.ofNat 64 (↑Main[22] + ↑Main[23] * 65536 + ↑Main[24] * 4294967296 + ↑Main[25] * 281474976710656)) := by
 
---   rw [run_readReg_bind, h_pc]
---   simp
---   stop
---   rw [run_readReg_bind]
---   simp
+    sorry
 
---   rw [Std.ExtDHashMap.get?_insert]
---   simp [h_pc]
+  cases h13_is_bool with
+  | inl h13_is_0 =>
+      simp [h13_is_0] at cstrs
+      have h6 : Main[6] ≠ 0 := by aesop
+      have h6_bv : BitVec.ofNat 5 ↑Main[6] = 0#5 := sorry
+      rw [run_readReg, read_pc]
+      simp [h6]
+      rw [run_readReg]
+      simp [Std.ExtDHashMap.get?_insert, read_pc, hmod]
+      rw [run_readReg]
+      simp [Std.ExtDHashMap.get?_insert, Std.ExtDHashMap.get?_eq_some_get h_misa]
+      rw [run_readReg]
+      simp [BitVec.ofNatLT_eq_ofNat, h6_bv]
+      simp [h_add]
 
---   simp [ext_control_check_pc]
+  | inr h13_is_1 =>
+      simp [h13_is_1] at cstrs
+      have h6 : Main[6] = 0 := by aesop
 
---   simp [bit_to_bool, bool_bit_backwards, Sail.BitVec.access, bits_of_virtaddr]
-
---   have : (BitVec.ofNat 64 (↑Main[3] + ↑Main[4] * 65536 + ↑Main[5] * 4294967296) +
---             sign_extend (BitVec.ofNat 21 (↑Main[14] + ↑Main[15] * 65536 + ↑Main[16] * 4294967296 + ↑Main[17] * 281474976710656)))[1] = false := sorry
-
---   simp [this, currentlyEnabled]
---   rw [run_readReg_bind]
---   simp
-
---   -- have := ext_control_check_pc
---   --         (BitVec.ofNat 64 (↑Main[3] + ↑Main[4] * 65536 + ↑Main[5] * 4294967296) +
---   --           sign_extend
---   --             (BitVec.ofNat 21
---   --               (↑Main[14] + ↑Main[15] * 65536 + ↑Main[16] * 4294967296 + ↑Main[17] * 281474976710656)))
-
---   simp [Std.ExtDHashMap.get?_insert, h_misa]
---   simp [get_next_pc]
---   rw [run_readReg_bind]
-
---   simp [LeanRV64IM.Functions.not, hartSupports]
-
---   simp [← SailState.wX_bits_is_regidx_write,
---     SailState.regidx_write]
-
---   by_cases h6 : Main[6] = 0
---   · simp [h6]
-
---     sorry
-
---   have h6' : BitVec.ofNat 5 Main[6] = 0#5 := sorry
---   simp [h6', EStateM.run_bind]
+      simp [h6]
+      rw [run_readReg]
+      simp [read_pc]
+      rw [run_readReg]
+      simp [Std.ExtDHashMap.get?_insert, read_pc, hmod]
+      rw [run_readReg]
+      simp [Std.ExtDHashMap.get?_insert, Std.ExtDHashMap.get?_eq_some_get h_misa]
+      rw [run_readReg]
+      simp [h_add]
 
 
-
---   have h25 : Main[25] = 0 := by
---     refine eq_zero_of_constraints Main h_cstrs
-
---   have h_imm :
---       BitVec.ofNat 64 (Main[22] + Main[23] * 65536 + Main[24] * 4294967296) =
---         BitVec.ofNat 64 (Main[3] + Main[4] * 65536 + ↑Main[5] * 4294967296) +
---           BitVec.ofNat 64 (Main[14] + Main[15] * 65536 + Main[16] * 4294967296 + Main[17] * 281474976710656) := by
---     refine add_imm_eq_of_constarints Main h_cstrs h_is_real
-
---   have h_of_int : let imm_nat : ℕ := Main[14] + Main[15] * 65536 + Main[16] * 4294967296 + Main[17] * 281474976710656
---       BitVec.ofInt 64 (BitVec.ofNat 21 (imm_nat)).toInt = (BitVec.ofNat 64 (imm_nat)) :=
---     ofInt_ofNat_of_constraints Main h_cstrs h_is_real
-
---   simp [h25]
-
---   have op_a_is_bool : Main[13] = 0 ∨ Main[13] = 1 := by
---     simp [constraints, h_is_real, SP1Constraint.toProp, Opcode.ofNat, Nat.ble] at h_cstrs
---     aesop
-
---   cases Or.symm op_a_is_bool with
---   | inl op_a_is_one =>
---       simp [constraints, op_a_is_one, h_is_real] at h_cstrs
---       have h26 : Main[26] = 0 := by aesop
---       have h27 : Main[27] = 0 := by aesop
---       have h28 : Main[28] = 0 := by aesop
---       have h29 : Main[29] = 0 := by aesop
---       have h6 : Main[6] = 0 := by
---         simp [SP1Constraint.toProp] at h_cstrs
---         simp_all only [BB_eq, Fin.isValue, Nat.reducePow]
---       simp_all
---       -- simp [h25, h26, h27, h28, h29, h6]
---       -- rw [h_imm]
---       -- simp only [set_next_pc, BB_eq, h_pc, Nat.reducePow, get_next_pc, sign_extend,
---       --   Sail.BitVec.signExtend, BitVec.signExtend, pure_bind, writeReg_readReg_bind,
---       --   writeReg_wX_bits_writeReg]
---       -- rw [h_of_int]
---       -- congr 3
-
---       -- sorry
---       -- unfold wX_bits
---       -- simp only [wX, BitVec.toNat_ofNat, Nat.reducePow, Nat.zero_mod, bne_self_eq_false, cond_false,
---       --   bind_pure_comp, map_pure, pure_bind, BB_eq]
---       -- rfl
---   | inr op_a_is_zero =>
-
---     have h_link : BitVec.ofNat 64 (Main[26] + Main[27] * 2^16 + Main[28] * 2^32 +  Main[29] * 2^48) =
---         BitVec.ofNat 64 (Main[3] + Main[4] * 2^16 + Main[5] * 2^32) + 4 := by
---       refine link_eq_of_constraints Main h_cstrs h_is_real op_a_is_zero
-
---     -- erw [h_link]
---     simp only [BB_eq, Nat.reducePow, BitVec.ofNat_eq_ofNat, set_next_pc, h25, Fin.isValue,
---       Fin.coe_ofNat_eq_mod, Nat.zero_mod, zero_mul, add_zero, h_pc, get_next_pc, sign_extend,
---       Sail.BitVec.signExtend, BitVec.signExtend, pure_bind, writeReg_readReg_bind,
---       writeReg_wX_bits_writeReg]
---     congr 1
-
---     simp [h_imm, h_of_int]
-
-
--- #print axioms SP1JAL_correct
 
 end JalChip
